More

CpcMini/Lemmas.lean
@@ -44,18 +44,31 @@ by
 
 /- Helper definitions -/
 
+def __eo_lem_state_to_formula_step : CStateObj -> Term -> Term
+  | CStateObj.assume F,
+      (Term.Apply (Term.Apply Term.imp F1) (Term.Apply (Term.Apply Term.imp F2) F3)) =>
+      (Term.Apply (Term.Apply Term.imp (Term.Apply (Term.Apply Term.and F) F1))
+        (Term.Apply (Term.Apply Term.imp F2) F3))
+  | CStateObj.assume_push F,
+      (Term.Apply (Term.Apply Term.imp F1) (Term.Apply (Term.Apply Term.imp F2) F3)) =>
+      (Term.Apply (Term.Apply Term.imp F1)
+        (Term.Apply (Term.Apply Term.imp (Term.Apply (Term.Apply Term.and F) F2)) F3))
+  | CStateObj.proven F,
+      (Term.Apply (Term.Apply Term.imp F1) (Term.Apply (Term.Apply Term.imp F2) F3)) =>
+      (Term.Apply (Term.Apply Term.imp F1)
+        (Term.Apply (Term.Apply Term.imp F2) (Term.Apply (Term.Apply Term.and F) F3)))
+  | _, _ => Term.Stuck
+
+
 def __eo_lem_state_to_formula_rec : CState -> Term -> Term
   | _ , Term.Stuck  => Term.Stuck
   | CState.nil, F => F
-  | (CState.cons (CStateObj.assume F) s), (Term.Apply (Term.Apply Term.imp F1) (Term.Apply (Term.Apply Term.imp F2) F3)) => (Term.Apply (Term.Apply Term.imp (Term.Apply (Term.Apply Term.and F) F1)) (Term.Apply (Term.Apply Term.imp F2) F3))
-  | (CState.cons (CStateObj.assume_push F) s), (Term.Apply (Term.Apply Term.imp F1) (Term.Apply (Term.Apply Term.imp F2) F3)) => (Term.Apply (Term.Apply Term.imp F1) (Term.Apply (Term.Apply Term.imp (Term.Apply (Term.Apply Term.and F) F2)) F3))
-  | (CState.cons (CStateObj.proven F) s), (Term.Apply (Term.Apply Term.imp F1) (Term.Apply (Term.Apply Term.imp F2) F3)) => (Term.Apply (Term.Apply Term.imp F1) (Term.Apply (Term.Apply Term.imp F2) (Term.Apply (Term.Apply Term.and F) F3)))
-  | s, F => Term.Stuck
+  | (CState.cons so s), F => (__eo_lem_state_to_formula_step so (__eo_lem_state_to_formula_rec s F))
+  | CState.Stuck, F => Term.Stuck
 
 
 def __eo_lem_state_to_formula (s : CState) : Term :=
   
     let _v0 := (Term.Apply Term.imp (Term.Boolean true))
     (__eo_lem_state_to_formula_rec s (Term.Apply _v0 (Term.Apply _v0 (Term.Boolean true))))
-
 
